fstar/MLS.TreeSync.Symbolic.LeafNodeSignature.fst
@@ -84,10 +84,9 @@ let tree_has_event_arithmetic_lemma l i =
 
 val tree_to_event:
   #tkt:treekem_types dy_bytes ->
-  #l:nat -> #i:tree_index l ->
-  mls_bytes dy_bytes -> treesync dy_bytes tkt l i ->
+  mls_bytes dy_bytes -> (l:nat & i:tree_index l & treesync dy_bytes tkt l i) ->
   event
-let tree_to_event #tkt #l #i group_id t =
+let tree_to_event #tkt group_id (|l, i, t|) =
   tree_has_event_arithmetic_lemma l i;
   let evt: group_has_tree_event dy_bytes tkt = {
     group_id;
@@ -100,7 +99,7 @@ let tree_to_event #tkt #l #i group_id t =
 
 val tree_has_event: #tkt:treekem_types dy_bytes -> principal -> timestamp -> mls_bytes dy_bytes -> (l:nat & i:tree_index l & treesync dy_bytes tkt l i) -> prop
 let tree_has_event #tkt prin time group_id (|l, i, t|) =
-  did_event_occur_before time prin (tree_to_event group_id t)
+  did_event_occur_before time prin (tree_to_event group_id (|l, i, t|))
 
 val tree_has_equivalent_event: #l:nat -> #i:tree_index l -> tkt:treekem_types dy_bytes -> principal -> timestamp -> mls_bytes dy_bytes -> treesync dy_bytes tkt l i -> leaf_index l i -> prop
 let tree_has_equivalent_event #l #i tkt prin time group_id t li =
